Refactor, add more theorems

src/register_machine.lean
@@ -9,15 +9,54 @@ import logic.function.iterate
 instance {α : Type*} [has_repr α] {len : ℕ} : has_repr (vector α len)
   := {repr := λ v, repr v.to_list}
 
+@[simp]
 lemma vector.update_nth_eq_if {α : Type*} {len : ℕ} {v : vector α len}
     {i : fin len} {elem : α} (h : v.nth i = elem)
-  : (v.update_nth i elem) = v
+  : v.update_nth i elem = v
   := begin
     refine vector.ext _,
     assume m,
     rw vector.nth_update_nth_eq_if,
     rw ← h,
-    sorry
+    split_ifs,
+    simp [h_1]
+  end
+
+@[simp]
+lemma vector.update_nth_update_nth_same {α : Type*} {len : ℕ} {v : vector α len}
+    {i : fin len} {e1 e2 : α}
+  : (v.update_nth i e1).update_nth i e2 = v.update_nth i e2
+  := begin
+    refine vector.ext _,
+    assume m,
+    by_cases i=m,
+    rw h,
+    iterate { rw vector.nth_update_nth_same },
+    iterate { rw vector.nth_update_nth_of_ne },
+    iterate { exact h }
+  end
+
+lemma vector.update_nth_comm {α : Type*} {len : ℕ} {v : vector α len}
+    {i j : fin len} {e1 e2 : α} (p : i ≠ j)
+  : (v.update_nth i e1).update_nth j e2 = (v.update_nth j e2).update_nth i e1
+  := begin
+    refine vector.ext _,
+    assume m,
+    by_cases i=m,
+    rw h,
+    rw vector.nth_update_nth_same,
+    rw vector.nth_update_nth_of_ne,
+    rw vector.nth_update_nth_same,
+    rw ← h,
+    exact ne.symm p,
+    by_cases j=m,
+    rw ← h,
+    rw vector.nth_update_nth_same,
+    rw vector.nth_update_nth_of_ne,
+    rw vector.nth_update_nth_same,
+    exact p,
+    iterate {rw vector.nth_update_nth_of_ne},
+    iterate {simp [*]},
   end
 
 namespace regmachine
@@ -48,51 +87,36 @@ end instr
 structure state (rc ic : ℕ) := (ip : option (fin ic)) (regs : vector ℕ rc)
 namespace state
   def is_halted {rc ic : ℕ} (s : state rc ic) := s.ip = none
+  def new_ic {rc ic ic' : ℕ} (s : state rc ic) : state rc (ic+ic') :=
+    { ip := s.ip.map (λ l, fin.cast_add ic' l), regs := s.regs }
 end state
 
 /- register machine with rc registers and ic instructions -/
 def rm (rc ic : ℕ)
   := vector (instr rc ic) ic
 
+/- most important definition here! gives semantics to those incs and decs :) -/
+def step {rc ic : ℕ} (M : rm rc ic) (c : state rc ic) : state rc ic :=
+  match c.ip with
+  | none := c
+  | some ip :=
+    match M.nth ip with
+    | instr.inc r l := {ip := l, regs := c.regs.update_nth r (c.regs.nth r + 1)}
+    | instr.dec r l k :=
+        match c.regs.nth r with
+        | p + 1 := {ip := l, regs := c.regs.update_nth r p}
+        | 0 := {ip := k, regs := c.regs}
+        end
+    end
+  end
+
 namespace rm
   variables {rc ic : ℕ}
-
-  section variable (M : rm rc ic)
-  def extend {n : ℕ} : rm (rc+n) ic
-    := M.map (instr.map_regs (fin.cast_add n))
-
-  def append {ic' : ℕ} (M' : rm rc ic'.succ)
-    : rm rc (ic + ic'.succ)
-    := vector.append
-        (M.map (instr.map_locs (λ l, match l with
-          | some l' := some (fin.cast_add ic' l')
-          | none := some ic
-          end)))
-        (M'.map (instr.map_locs (λ l, match l with
-          | some l' := some (ic + l')
-          | none := none
-          end)))
-
-  /- most important definition here! gives semantics to those incs and decs :) -/
-  def step (c : state rc ic) : state rc ic :=
-    match c.ip with
-    | none := c
-    | some ip :=
-      match M.nth ip with
-      | instr.inc r l := {ip := l, regs := c.regs.update_nth r (c.regs.nth r + 1)}
-      | instr.dec r l k :=
-          match c.regs.nth r with
-          | p + 1 := {ip := l, regs := c.regs.update_nth r p}
-          | 0 := {ip := k, regs := c.regs}
-          end
-      end
-    end
-
-  end
 
   /- a configuration for M is just a state.
       used to store M at the type level. -/
   structure conf (M : rm rc ic) := (s : state rc ic)
+
   @[simp]
   def mk_conf (M : rm rc ic) (s : state rc ic) : M.conf := {s := s}
 
@@ -100,22 +124,54 @@ namespace rm
     variables {M : rm rc ic} (c : M.conf)
 
     def steps_to (d : M.conf) :=
-      ∃ (t : ℕ), (M.step)^[t] c.s = d.s
+      ∃ (t : ℕ), (step M)^[t] c.s = d.s
 
     notation c `==>` d := c.steps_to d
 
-    theorem steps_to_trans (c d e : M.conf)
+    lemma step_is_steps_to {c d : state rc ic}
+      (pf : step M c = d) : M.mk_conf c ==> conf.mk d
+      := begin use 1, simpa end
+
+    lemma steps_to_trans (c d e : M.conf)
       (pf1 : c ==> d) (pf2 : d ==> e) : c ==> e
       := begin
         cases pf1,
         cases pf2,
         use pf2_w + pf1_w,
-        simp [function.iterate_add],
-        rw pf1_h,
-        exact pf2_h
+        simpa [function.iterate_add, pf1_h]
       end
 
   end conf
+
+  section variable (M : rm rc ic)
+
+  def extend {n : ℕ} : rm (rc+n) ic
+    := M.map (instr.map_regs (fin.cast_add n))
+
+  /- joins M with M', one set of instructions
+    after the other. allows the "rewiring"
+    of the halts in each machine to a new loc
+    in the new machine -/
+  def join {ic' : ℕ} (M_halt_loc : option (fin (ic + ic')))
+          (M' : rm rc ic') (M'_halt_loc : option (fin (ic + ic')))
+    : rm rc (ic + ic')
+    := vector.append
+        (M.map (instr.map_locs (λ lopt, match lopt with
+          | some l := some (⟨l.val + ic', begin simpa using l.property end⟩)
+          | none := M_halt_loc
+          end)))
+        (M'.map (instr.map_locs (λ lopt, match lopt with
+          | some l := some (⟨ic + l.val, begin simpa using l.property end⟩)
+          | none := M'_halt_loc
+          end)))
+
+  theorem join_preserves_behavior_fst  {ic' : ℕ} (M_halt_loc  : option (fin (ic + ic')))
+          (M' : rm rc ic') (M'_halt_loc : option (fin (ic + ic')))
+    : ∀ {c d : M.conf} (h : c ==> d),
+        (M.join M_halt_loc M' M'_halt_loc).mk_conf c.s.new_ic ==> conf.mk d.s.new_ic
+    := begin sorry end
+  
+  end
 
   open conf
 
@@ -135,46 +191,90 @@ variables {rc ic : ℕ}
   open instr
   open rm
 
+  -- sets register r back to 0
   def rst (r : fin rc) : rm rc 1 := ⟨[
     dec r (some 0) none
   ], rfl⟩
 
-  lemma rst_step (r : fin rc) {n : ℕ} {regs : vector ℕ rc} {h : regs.nth r = n.succ}
-    : (rst r).step {ip := some 0, regs := regs} =
-      {ip := some 0, regs := regs.update_nth r n}
-    := begin
-      simp [rst, step, vector.head],
-      rw h,
-      simpa
-    end
+  section
+  variables {r : fin rc} {regs : vector ℕ rc}
 
-  theorem rst_effect {r : fin rc} {n : ℕ} {regs : vector ℕ rc} {h : regs.nth r = n}
+  lemma rst_step_zero (h : regs.nth r = 0)
+    : (rst r).mk_conf {ip := some 0, regs := regs} ==>
+        conf.mk {ip := none, regs := regs}
+    := begin apply conf.step_is_steps_to, simp [step, vector.head, rst, h] end
+  
+  lemma rst_step_succ {n : ℕ} (h : regs.nth r = n.succ)
+    : (rst r).mk_conf {ip := some 0, regs := regs} ==>
+        conf.mk {ip := some 0, regs := regs.update_nth r n}
+    := begin apply conf.step_is_steps_to, simp [step, vector.head, rst, h] end
+  
+  theorem rst_effect {r : fin rc} {regs : vector ℕ rc}
     : (rst r).mk_conf {ip := some 0, regs := regs} ==>
       conf.mk {ip := none, regs := regs.update_nth r 0}
     := begin
-      rw conf.steps_to,
-      use n.succ,
-      simp,
-      induction n,
-      simp [nat.iterate, step, vector.head, rst],
-      rw h,
-      rw vector.update_nth_eq_if,
-      simp [step],
-      exact h,
-      sorry
+      induction h : (regs.nth r) generalizing regs,
+      simp [step, h],
+      exact rst_step_zero h,
+      refine rm.conf.steps_to_trans _
+        ((rst r).mk_conf {ip := some 0, regs := regs.update_nth r n})
+        _ _ _,
+      exact rst_step_succ h,
+      have : (regs.update_nth r n).nth r = n := vector.nth_update_nth_same _ _ _,
+      convert ih this using 3,
+      rw vector.update_nth_update_nth_same
     end
+
+  end
 
   def mov (_from _to : fin rc) : rm rc 2 := ⟨[
     dec _from (some 1) none,
     inc _to (some 0)
   ], rfl⟩
   
-  theorem mov_effect {_from _to : fin rc} {rs : vector ℕ rc} {p : _from ≠ _to}
-    : (mov _from _to).mk_conf {ip := some 0, regs := rs} ==>
-      conf.mk {ip := none, regs := (rs.update_nth _from 0).update_nth _to (rs.nth _from + rs.nth _to)}
+  section
+  variables {_from _to : fin rc} {regs : vector ℕ rc}
+
+  lemma mov_step_zero (h : regs.nth _from = 0)
+    : (mov _from _to).mk_conf {ip := some 0, regs := regs} ==>
+        conf.mk {ip := none, regs := regs}
+    := begin apply rm.conf.step_is_steps_to, simp [step, vector.head, mov, h] end
+  
+  lemma mov_step_succ {n_to n_from : ℕ} {nonequal : ¬ _from = _to} (h_from : regs.nth _from = n_from.succ) (h_to : regs.nth _to = n_to)
+    : (mov _from _to).mk_conf {ip := some 0, regs := regs} ==>
+        conf.mk {ip := some 0, regs := (regs.update_nth _from n_from).update_nth _to n_to.succ}
     := begin
-      sorry
+        simp,
+        use 2,
+        simp [step, vector.head, vector.nth, mov, h_from, h_to, vector.nth_update_nth_of_ne nonequal]
+      end
+
+  theorem mov_effect {nonequal : ¬ _from = _to}
+    : (mov _from _to).mk_conf {ip := some 0, regs := regs} ==>
+      conf.mk {ip := none, regs := (regs.update_nth _from 0).update_nth _to (regs.nth _from + regs.nth _to)}
+    := begin
+      induction h : (regs.nth _from) generalizing regs,
+      simp [step, h],
+      exact mov_step_zero h,
+      refine rm.conf.steps_to_trans _
+        ((mov _from _to).mk_conf {ip := some 0, regs :=  (regs.update_nth _from n).update_nth _to (regs.nth _to).succ})
+        _ _ _,
+      refine mov_step_succ h rfl,
+      exact nonequal,
+      have : ((regs.update_nth _from n).update_nth _to (regs.nth _to).succ).nth _from = n,
+      rw vector.nth_update_nth_of_ne,
+      apply vector.nth_update_nth_same,
+      exact ne.symm nonequal,
+      convert ih this using 3,
+      simp [vector.nth_update_nth_of_ne],
+      rw vector.update_nth_comm (ne.symm nonequal),
+      simp [vector.update_nth_update_nth_same],
+      suffices : n.succ + regs.nth _to = n + (regs.nth _to).succ,
+        rw this,
+      exact nat.succ_add n (vector.nth regs _to)
     end
+
+  end
 
 end macros
 
